{"cells":[{"cell_type":"markdown","metadata":{},"source":["## TMA4215 - Project #1 ## \n","*27.09.2024*\n","\n","*Candidate ID*"]},{"cell_type":"markdown","metadata":{},"source":["In this project I have used numerical methods for Fourier series based signal processing."]},{"cell_type":"code","execution_count":5,"metadata":{},"outputs":[],"source":["import numpy as np\n","import matplotlib.pyplot as plt\n","from numba import jit, njit"]},{"cell_type":"markdown","metadata":{},"source":["#### Task 1: The (Discrete) Fourier Transform"]},{"cell_type":"markdown","metadata":{},"source":["#### a)\n","\n","Considering the functions $e^{2\\pi ikx}$, $k \\in \\mathbb{Z}$, $x \\in \\mathbb{T}$. I am going to below prove that for any $k, h \\in \\mathbb{Z}$ we have\n","\n","$$\n","\\left\\langle e^{2\\pi i k \\cdot}, e^{2\\pi i h \\cdot} \\right\\rangle = \n","\\begin{cases} \n","1 & \\text{if } k = h \\\\\n","0 & \\text{else}\n","\\end{cases}\n","$$\n","\n","\n","The inner product of two functions $f(x)$ and $g(x)$ on the interval $[0, 1)$ is defined as:\n","\n","$$\n","\\langle f, g \\rangle = \\int_0^1 f(x) \\overline{g(x)} \\, dx\n","$$\n","\n","For our case, $f(x) = e^{2\\pi i k x}$ and $g(x) = e^{2\\pi i h x}$. The complex conjugate of $g(x)$ is:\n","\n","$$\n","\\overline{g(x)} = e^{-2\\pi i h x}\n","$$\n","\n","Thus, the inner product becomes:\n","\n","$$\n","\\langle e^{2\\pi i k x}, e^{2\\pi i h x} \\rangle = \\int_0^1 e^{2\\pi i k x} \\cdot e^{-2\\pi i h x} \\, dx = \\int_0^1 e^{2\\pi i (k - h) x} \\, dx\n","$$\n","\n","We have two cases:\n","\n","1. **$k = h$:**\n","\n","$$\n","\\int_0^1 e^{2\\pi i (k - h) x} \\, dx = \\int_0^1 e^{0} \\, dx = \\int_0^1 1 \\, dx = 1\n","$$\n","\n","So, the inner product is 1 when $k = h$.\n","\n","2. **$k \\neq h$:**\n","\n","In this case, let $m = k - h \\neq 0$. We need to evaluate:\n","\n","$$\n","\\int_0^1 e^{2\\pi i m x} \\, dx\n","$$\n","\n","The antiderivative of $e^{2\\pi i m x}$ is:\n","\n","$$\n","\\int e^{2\\pi i m x} \\, dx = \\frac{e^{2\\pi i m x}}{2\\pi i m}\n","$$\n","\n","Evaluating this from $0$ to $1$ gives:\n","\n","$$\n","\\left[ \\frac{e^{2\\pi i m x}}{2\\pi i m} \\right]_0^1 = \\frac{e^{2\\pi i m \\cdot 1} - e^{2\\pi i m \\cdot 0}}{2\\pi i m} = \\frac{e^{2\\pi i m} - 1}{2\\pi i m}\n","$$\n","\n","Since $e^{2\\pi i m} = 1$ for any integer $m$, we have:\n","\n","$$\n","\\frac{1 - 1}{2\\pi i m} = 0\n","$$\n","\n","So, the inner product is $0$ when $k \\neq h$.\n","\n","$\\square$\n"]},{"cell_type":"markdown","metadata":{},"source":["#### b)\n","\n","Now considering the functions of the form $\\sqrt{2} \\sin(2\\pi mx)$, $m = 1, 2, \\ldots$, $\\cos(2\\pi 0 x)$, and $\\sqrt{2} \\cos(2\\pi nx)$, $n = 1, 2, \\ldots$, $x \\in \\mathbb{T}$. I want to prove that these form an orthonormal system.\n","\n","1. **Orthogonality between sine and cosine functions:**\n","\n","The inner product of $\\sqrt{2} \\sin(2\\pi n x)$ and $\\sqrt{2} \\cos(2\\pi m x)$ is given by:\n","\n","$$\n","\\langle \\sqrt{2} \\sin(2\\pi n x), \\sqrt{2} \\cos(2\\pi m x) \\rangle = 2 \\int_0^1 \\sin(2\\pi n x) \\cos(2\\pi m x) \\, dx\n","$$\n","\n","Using the trigonometric identity:\n","\n","$$\n","\\sin A \\cos B = \\frac{1}{2} [\\sin(A + B) + \\sin(A - B)],\n","$$\n","\n","we get:\n","\n","$$\n","2 \\int_0^1 \\sin(2\\pi n x) \\cos(2\\pi m x) \\, dx = \\int_0^1 [\\sin(2\\pi (n+m) x) + \\sin(2\\pi (n-m) x)] \\, dx\n","$$\n","\n","Both integrals of $\\sin(2\\pi k x)$ over the interval $[0, 1]$ are zero because the sine function completes an integer number of periods, and its average value over a full period is zero. Therefore, the inner product is also zero. Hence:\n","\n","$$\n","\\langle \\sqrt{2} \\sin(2\\pi n \\cdot), \\sqrt{2} \\cos(2\\pi m \\cdot) \\rangle = 0, \\quad n \\in \\{1, 2, \\ldots\\}, \\, m \\in \\{0, 1, \\ldots\\}\n","$$\n","\n","2. **Orthogonality and normality between two sine functions:**\n","\n","The inner product of $\\sqrt{2} \\sin(2\\pi n x)$ and $\\sqrt{2} \\sin(2\\pi m x)$ is:\n","\n","$$\n","\\langle \\sqrt{2} \\sin(2\\pi n x), \\sqrt{2} \\sin(2\\pi m x) \\rangle = 2 \\int_0^1 \\sin(2\\pi n x) \\sin(2\\pi m x) \\, dx\n","$$\n","\n","Using the identity:\n","\n","$$\n","\\sin A \\sin B = \\frac{1}{2} [\\cos(A - B) - \\cos(A + B)],\n","$$\n","\n","we get:\n","\n","$$\n","2 \\int_0^1 \\sin(2\\pi n x) \\sin(2\\pi m x) \\, dx = \\int_0^1 [\\cos(2\\pi (n-m) x) - \\cos(2\\pi (n+m) x)] \\, dx\n","$$\n","\n","The integral of $\\cos(2\\pi k x)$ over $[0, 1]$ is zero for any integer $k \\neq 0$. For $k = 0$ (when $n = m$), the integral of $1$ over $[0, 1]$ is $1$. Hence, the inner product is $1$ if $n = m$ and $0$ otherwise. So:\n","\n","$$\n","\\langle \\sqrt{2} \\sin(2\\pi n \\cdot), \\sqrt{2} \\sin(2\\pi m \\cdot) \\rangle = \n","\\begin{cases} \n","0 & \\text{if } m \\neq n \\\\\n","1 & \\text{if } m = n \n","\\end{cases}, \\quad m, n \\in \\{1, 2, \\ldots\\}\n","$$\n","\n","3. **Orthogonality and normality between two cosine functions:**\n","\n","The inner product of $\\sqrt{2} \\cos(2\\pi n x)$ and $\\sqrt{2} \\cos(2\\pi m x)$ is:\n","\n","$$\n","\\langle \\sqrt{2} \\cos(2\\pi n x), \\sqrt{2} \\cos(2\\pi m x) \\rangle = 2 \\int_0^1 \\cos(2\\pi n x) \\cos(2\\pi m x) \\, dx\n","$$\n","\n","Using the identity:\n","\n","$$\n","\\cos A \\cos B = \\frac{1}{2} [\\cos(A + B) + \\cos(A - B)],\n","$$\n","\n","we get:\n","\n","$$\n","2 \\int_0^1 \\cos(2\\pi n x) \\cos(2\\pi m x) \\, dx = \\int_0^1 [\\cos(2\\pi (n + m) x) + \\cos(2\\pi (n - m) x)] \\, dx\n","$$\n","\n","The integral of $\\cos(2\\pi k x)$ over $[0, 1]$ is zero for any integer $k \\neq 0$. For $k = 0$ (when $n = m$), the integral of $1$ over $[0, 1]$ is $1$. For $n = m = 0$, the integral of $1$ over $[0, 1]$ multiplied by $2$ is $2$. Hence, the inner product is $2$ if $n = m = 0$, $1$ if $n = m \\neq 0$, and $0$ otherwise. Which we can write as:\n","\n","$$\n","\\langle \\sqrt{2} \\cos(2\\pi n \\cdot), \\sqrt{2} \\cos(2\\pi m \\cdot) \\rangle = \n","\\begin{cases} \n","0 & \\text{if } m \\neq n \\\\\n","1 & \\text{if } m = n \\neq 0 \\\\\n","2 & \\text{if } m = n = 0 \n","\\end{cases}, \\quad m, n \\in \\{0, 1, \\ldots\\}\n","$$\n","\n","$\\square$\n"]},{"cell_type":"markdown","metadata":{},"source":["#### c)\n","\n","Now we introduce the following two spaces, $T_n$ and $S_n$:\n","\n","$$\n","T_n := \\text{span}(e^{-2\\pi in\\cdot}, \\ldots, e^{2\\pi in\\cdot}) = \\left\\{ f \\, \\middle| \\, f(x) = \\sum_{k=-n}^{n} c_k e^{2\\pi ikx}, \\, \\text{where } c_{-n}, c_{-n+1}, \\ldots, c_n \\in \\mathbb{C} \\right\\}\n","$$\n","\n","$$\n","S_n := \\text{span}(\\cos(0\\cdot), \\cos(2\\pi\\cdot), \\ldots, \\cos(2\\pi n\\cdot), \\sin(2\\pi\\cdot), \\sin(2\\pi \\cdot 2), \\ldots, \\sin(2\\pi n\\cdot))\n","$$\n","\n","$$\n","= \\left\\{ f \\, \\middle| \\, f(x) = \\frac{a_0}{2} + \\sum_{k=1}^{n} a_k \\cos(2\\pi kx) + b_k \\sin(2\\pi kx), \\, \\text{where } a_0, a_1, \\ldots, a_n, b_1, \\ldots, b_n \\in \\mathbb{R} \\right\\}\n","$$\n","\n","Using the results from Item a) and b) I want to find orthonormal bases for these two spaces.\n","\n","**Orthonormal basis for $T_n$:**\n","\n","From Item a), we have shown that the functions $e^{2\\pi i k \\cdot}$ for $k = -n, \\ldots, n$ form an orthonormal set on the interval $[0, 1)$. To construct an orthonormal basis for $T_n$, we consider the set:\n","\n","$$\n","\\left\\{ e^{2\\pi i k x} \\, \\middle| \\, k = -n, \\ldots, n \\right\\}\n","$$\n","\n","Thus, the orthonormal basis for $T_n$ is:\n","\n","$$\n","\\left\\{ e^{2\\pi i k x} \\, \\middle| \\, k = -n, \\ldots, n \\right\\}\n","$$\n","\n","**Orthonormal basis for $S_n$:**\n","\n","From Item b), we have shown the orthogonality properties of the sine and cosine functions. We can use the results to form orthonormal bases for $S_n$.\n","\n","- **For Cosine Functions:**\n","\n","The function $\\cos(0)$ is not normalized, so we use $1$ instead of $\\cos(0)$. For $k = 1, \\ldots, n$, the normalized cosine functions are $\\sqrt{2} \\cos(2\\pi k x)$.\n","\n","The orthonormal basis for the cosine components is:\n","\n","$$\n","\\left\\{ 1, \\sqrt{2} \\cos(2\\pi k x) \\, \\middle| \\, k = 1, 2, \\ldots, n \\right\\}\n","$$\n","\n","- **For Sine Functions:**\n","\n","For $k = 1, \\ldots, n$, the normalized sine functions are $\\sqrt{2} \\sin(2\\pi k x)$.\n","\n","The orthonormal basis for the sine components is:\n","\n","$$\n","\\left\\{ \\sqrt{2} \\sin(2\\pi k x) \\, \\middle| \\, k = 1, 2, \\ldots, n \\right\\}\n","$$\n","\n","\n","**Proving $T_n = S_n$ Using Euler's Identity:**\n","\n","Euler's identity states:\n","\n","$$\n","e^{i\\theta} = \\cos(\\theta) + i\\sin(\\theta)\n","$$\n","\n","Using this, we can express the exponential functions in $T_n$ in terms of sines and cosines:\n","\n","$$\n","e^{2\\pi ikx} = \\cos(2\\pi kx) + i\\sin(2\\pi kx)\n","$$\n","\n","$$\n","e^{-2\\pi ikx} = \\cos(2\\pi kx) - i\\sin(2\\pi kx)\n","$$\n","\n","Therefore, any function $f(x)$ in $T_n$ can be written as:\n","\n","$$\n","f(x) = \\sum_{k=-n}^{n} c_k e^{2\\pi ikx} = c_0 + \\sum_{k=1}^{n} c_k e^{2\\pi ikx} + c_{-k} e^{-2\\pi ikx}\n","$$\n","\n","Substituting the identities:\n","\n","$$\n","f(x) = c_0 + \\sum_{k=1}^{n} \\left[ c_k (\\cos(2\\pi kx) + i\\sin(2\\pi kx)) + \\overline{c_k} (\\cos(2\\pi kx) - i\\sin(2\\pi kx)) \\right]\n","$$\n","\n","$$\n","f(x) = c_0 + \\sum_{k=1}^{n} \\left[ (c_k + \\overline{c_k}) \\cos(2\\pi kx) + i(c_k - \\overline{c_k}) \\sin(2\\pi kx) \\right]\n","$$\n","\n","Since $c_k = \\overline{c_{-k}}$, we can set $c_k + \\overline{c_k} = 2\\Re(c_k) = a_k$ and $i(c_k - \\overline{c_k}) = 2i \\Im(c_k) = b_k$. This transforms the expression into:\n","\n","$$\n","f(x) = c_0 + \\sum_{k=1}^{n} a_k \\cos(2\\pi kx) + b_k \\sin(2\\pi kx)\n","$$\n","\n","This is precisely the form of the function in $S_n$. Therefore, every function in $T_n$ can be represented as a function in $S_n$. Conversely, any function in $S_n$ can be represented in terms of the exponential form of $T_n$. Hence, $T_n = S_n$.\n","\n","**Dimension of $T_n$:**\n","\n","The dimension of $T_n$ is the number of linearly independent basis functions. The basis functions for $T_n$ are $e^{-2\\pi inx}, e^{-2\\pi i(n-1)x}, \\ldots, e^{2\\pi inx}$.\n","\n","Since there are $2n + 1$ such basis functions, the dimension of $T_n$ is:\n","\n","$$\n","\\text{dim}(T_n) = 2n + 1\n","$$\n"]},{"cell_type":"markdown","metadata":{},"source":["#### d)\n","\n","From Item c), any function $ f(x) \\in S_n $ can be expressed as:\n","\n","$$\n","f(x) = \\frac{a_0}{2} + \\sum_{k=1}^{n} a_k \\cos(2\\pi kx) + b_k \\sin(2\\pi kx)\n","$$\n","\n","where $ a_0, a_1, \\ldots, a_n $ and $ b_1, \\ldots, b_n $ are the Fourier coefficients.\n","\n","This representation decomposes any function in $S_n$ into a finite sum of simpler trigonometric functions.\n","\n","The inner product on the space $S_n$ is defined as:\n","\n","$$\n","\\langle f, g \\rangle = \\int_{-\\frac{1}{2}}^{\\frac{1}{2}} f(x) g(x) \\, dx\n","$$\n","\n","We know from previously that the set of functions:\n","\n","$$\n","\\{ 1, \\sqrt{2} \\cos(2\\pi kx), \\sqrt{2} \\sin(2\\pi kx) \\, \\mid \\, k = 1, 2, \\ldots, n \\}\n","$$\n","\n","forms an orthonormal basis for $S_n$.\n","\n","Taking the inner product of $f(x)$ with each of these basis functions allows us to isolate each Fourier coefficient.\n","\n","To find $ a_k $, we take the inner product of $ f(x) $ with $ \\cos(2\\pi kx) $:\n","\n","$$\n","\\langle f, \\cos(2\\pi k \\cdot) \\rangle = \\int_{-\\frac{1}{2}}^{\\frac{1}{2}} f(x) \\cos(2\\pi kx) \\, dx\n","$$\n","\n","Now we substitute the representation of $ f(x) $ into this integral:\n","\n","$$\n","\\langle f, \\cos(2\\pi k \\cdot) \\rangle = \\int_{-\\frac{1}{2}}^{\\frac{1}{2}} \\left( \\frac{a_0}{2} + \\sum_{j=1}^{n} a_j \\cos(2\\pi jx) + b_j \\sin(2\\pi jx) \\right) \\cos(2\\pi kx) \\, dx\n","$$\n","\n","\n","$$\n","\\langle f, \\cos(2\\pi k \\cdot) \\rangle = \\int_{-\\frac{1}{2}}^{\\frac{1}{2}} \\frac{a_0}{2} \\cos(2\\pi kx) \\, dx + \\sum_{j=1}^{n} a_j \\int_{-\\frac{1}{2}}^{\\frac{1}{2}} \\cos(2\\pi jx) \\cos(2\\pi kx) \\, dx + \\sum_{j=1}^{n} b_j \\int_{-\\frac{1}{2}}^{\\frac{1}{2}} \\sin(2\\pi jx) \\cos(2\\pi kx) \\, dx\n","$$\n","\n","Using orthogonality properties:\n","\n","1. **Orthogonality of cosine with cosine:**\n","\n","$$\n","\\int_{-\\frac{1}{2}}^{\\frac{1}{2}} \\cos(2\\pi jx) \\cos(2\\pi kx) \\, dx = \n","\\begin{cases}\n","\\frac{1}{2} & \\text{if } j = k \\\\\n","0 & \\text{if } j \\neq k\n","\\end{cases}\n","$$\n","\n","2. **Orthogonality of sine with cosine:**\n","\n","$$\n","\\int_{-\\frac{1}{2}}^{\\frac{1}{2}} \\sin(2\\pi jx) \\cos(2\\pi kx) \\, dx = 0 \\quad \\forall j, k\n","$$\n","\n","This simplifies the expression for $ \\langle f, \\cos(2\\pi k \\cdot) \\rangle $ to:\n","\n","$$\n","\\langle f, \\cos(2\\pi k \\cdot) \\rangle = \\frac{a_k}{2}\n","$$\n","\n","Where we have:\n","\n","$$\n","a_k = 2 \\langle f, \\cos(2\\pi k \\cdot) \\rangle = 2 \\int_{-\\frac{1}{2}}^{\\frac{1}{2}} f(x) \\cos(2\\pi kx) \\, dx\n","$$\n","\n","for $ k = 0, 1, \\ldots, n $.\n","\n","The orthogonality property of the cosine functions allows all other terms in the series expansion of $ f(x) $ to cancel out, leaving only the $ a_k $ term.\n","\n","Furthermore, to find $ b_k $, we take the inner product of $ f(x) $ with $ \\sin(2\\pi kx) $:\n","\n","$$\n","\\langle f, \\sin(2\\pi k \\cdot) \\rangle = \\int_{-\\frac{1}{2}}^{\\frac{1}{2}} f(x) \\sin(2\\pi kx) \\, dx\n","$$\n","\n","Substituting the representation of $ f(x) $ into the integral:\n","\n","$$\n","\\langle f, \\sin(2\\pi k \\cdot) \\rangle = \\int_{-\\frac{1}{2}}^{\\frac{1}{2}} \\left( \\frac{a_0}{2} + \\sum_{j=1}^{n} a_j \\cos(2\\pi jx) + b_j \\sin(2\\pi jx) \\right) \\sin(2\\pi kx) \\, dx\n","$$\n","\n","Expanding:\n","\n","$$\n","\\langle f, \\sin(2\\pi k \\cdot) \\rangle = \\int_{-\\frac{1}{2}}^{\\frac{1}{2}} \\frac{a_0}{2} \\sin(2\\pi kx) \\, dx + \\sum_{j=1}^{n} a_j \\int_{-\\frac{1}{2}}^{\\frac{1}{2}} \\cos(2\\pi jx) \\sin(2\\pi kx) \\, dx + \\sum_{j=1}^{n} b_j \\int_{-\\frac{1}{2}}^{\\frac{1}{2}} \\sin(2\\pi jx) \\sin(2\\pi kx) \\, dx\n","$$\n","\n","Using orthogonality properties:\n","\n","1. **Orthogonality of cosine with sine:**\n","\n","$$\n","\\int_{-\\frac{1}{2}}^{\\frac{1}{2}} \\cos(2\\pi jx) \\sin(2\\pi kx) \\, dx = 0 \\quad \\forall j, k\n","$$\n","\n","2. **Orthogonality of sine with sine:**\n","\n","$$\n","\\int_{-\\frac{1}{2}}^{\\frac{1}{2}} \\sin(2\\pi jx) \\sin(2\\pi kx) \\, dx = \n","\\begin{cases}\n","\\frac{1}{2} & \\text{if } j = k \\\\\n","0 & \\text{if } j \\neq k\n","\\end{cases}\n","$$\n","\n","This simplifies the expression for $ \\langle f, \\sin(2\\pi k \\cdot) \\rangle $ to:\n","\n","$$\n","\\langle f, \\sin(2\\pi k \\cdot) \\rangle = \\frac{b_k}{2}\n","$$\n","\n","So,\n","\n","$$\n","b_k = 2 \\langle f, \\sin(2\\pi k \\cdot) \\rangle = 2 \\int_{-\\frac{1}{2}}^{\\frac{1}{2}} f(x) \\sin(2\\pi kx) \\, dx\n","$$\n","\n","for $ k = 1, \\ldots, n $.\n","\n","Here the orthogonality property of the sine functions allows all other terms in the series expansion of $ f(x) $ to drop out, leaving only the $ b_k $ term.\n","\n","Hence, we have shown that the Fourier coefficients $ a_k $ and $ b_k $ can be computed as:\n","\n","$$\n","a_k = 2 \\int_{-\\frac{1}{2}}^{\\frac{1}{2}} f(x) \\cos(2\\pi kx) \\, dx, \\quad k = 0, 1, \\ldots, n\n","$$\n","\n","$$\n","b_k = 2 \\int_{-\\frac{1}{2}}^{\\frac{1}{2}} f(x) \\sin(2\\pi kx) \\, dx, \\quad k = 1, \\ldots, n\n","$$\n","\n","$\\square$"]},{"cell_type":"markdown","metadata":{},"source":["#### e)\n","\n","Using equidistant points $ x_0, \\ldots, x_{N-1} $, where $ x_j = \\frac{j}{N} $, $ j = 0, \\ldots, N-1 $, for some $ N \\in \\mathbb{N} $, I want to approximate the integral required for the Fourier coefficients $c_k(f)$ of a function $f$. Note that the notation $ f_j = f(x_j) $ and $ \\mathbf{f} = (f_0, \\ldots, f_{N-1}) $ holds for simplicity.\n","\n","The Fourier coefficient $c_k(f)$ is defined as:\n","\n","$$\n","c_k(f) = \\int_{0}^{1} f(x) e^{-2\\pi i k x} \\, dx.\n","$$\n","\n","The trapezoidal rule is a numerical integration method that approximates the area under a curve by dividing it into trapezoids. To approximate this integral, we will use the composite trapezoidal rule with equidistant points $ x_j = \\frac{j}{N} $, where $ j = 0, 1, \\ldots, N-1 $.\n","\n","The trapezoidal rule approximation is given by:\n","\n","$$\n","c_k(f) \\approx \\hat{f}_k = \\frac{1}{N} \\sum_{j=0}^{N-1} f_j e^{-2\\pi i jk / N}\n","$$\n","\n","where $ f_j = f(x_j) = f\\left(\\frac{j}{N}\\right) $.\n","\n","Now we want to show $N$-Periodicity of $ \\hat{f}_k $\n","\n","In other words, we want to show that:\n","\n","$$\n","\\hat{f}_{k+N} = \\hat{f}_k.\n","$$\n","\n","Substituting $k+N$ into the formula for $ \\hat{f}_k $:\n","\n","$$\n","\\hat{f}_{k+N} = \\frac{1}{N} \\sum_{j=0}^{N-1} f_j e^{-2\\pi i j(k+N) / N}.\n","$$\n","\n","Simplifying the exponent:\n","\n","$$\n","\\hat{f}_{k+N} = \\frac{1}{N} \\sum_{j=0}^{N-1} f_j e^{-2\\pi i jk / N} e^{-2\\pi i j}.\n","$$\n","\n","Since $ e^{-2\\pi i j} = 1 $ for any integer $ j $, we have:\n","\n","$$\n","\\hat{f}_{k+N} = \\frac{1}{N} \\sum_{j=0}^{N-1} f_j e^{-2\\pi i jk / N} = \\hat{f}_k.\n","$$\n","\n","This shows that the coefficients $ \\hat{f}_k $ are $ N $-periodic, meaning that:\n","\n","$$\n","\\hat{f}_{k+N} = \\hat{f}_k \\quad \\forall k \\in \\mathbb{Z}.\n","$$\n","\n","The periodicity of $ \\hat{f}_k $ implies that the DFT, which uses these coefficients, assumes the original function $ f(x) $ is periodic with period $ 1 $ (the interval $[0, 1)$). If $ f(x) $ is not truly periodic with period $ 1 $, the periodicity of the DFT coefficients can cause *aliasing*, where higher frequencies in the original function are misrepresented in the approximation. The approximation of the Fourier coefficients using $ \\hat{f}_k $ involves a truncation error due to the finite number of points $ N $. As $ N $ increases, this error decreases, and the approximation becomes more accurate."]},{"cell_type":"markdown","metadata":{},"source":["#### f)"]},{"cell_type":"markdown","metadata":{},"source":["#### g)"]},{"cell_type":"markdown","metadata":{},"source":["#### h)"]},{"cell_type":"markdown","metadata":{},"source":["#### i)"]},{"cell_type":"markdown","metadata":{},"source":["#### j)"]},{"cell_type":"markdown","metadata":{},"source":["#### Task 2: Signal Processing"]},{"cell_type":"markdown","metadata":{},"source":["#### a)"]},{"cell_type":"markdown","metadata":{},"source":["#### b)"]},{"cell_type":"markdown","metadata":{},"source":["#### c)"]},{"cell_type":"markdown","metadata":{},"source":["#### d)"]},{"cell_type":"markdown","metadata":{},"source":["#### e)"]},{"cell_type":"markdown","metadata":{},"source":["#### Task 3: Sound Processing"]},{"cell_type":"markdown","metadata":{},"source":["#### a)"]},{"cell_type":"markdown","metadata":{},"source":["#### b)"]},{"cell_type":"markdown","metadata":{},"source":["#### c)"]},{"cell_type":"markdown","metadata":{},"source":["#### d)"]},{"cell_type":"markdown","metadata":{},"source":["#### e)"]},{"cell_type":"markdown","metadata":{},"source":["#### f)"]},{"cell_type":"markdown","metadata":{},"source":["#### g)"]},{"cell_type":"markdown","metadata":{},"source":[]}],"metadata":{"kernelspec":{"display_name":"3.12","language":"python","name":"python3"},"language_info":{"codemirror_mode":{"name":"ipython","version":3},"file_extension":".py","mimetype":"text/x-python","name":"python","nbconvert_exporter":"python","pygments_lexer":"ipython3","version":"3.12.2"}},"nbformat":4,"nbformat_minor":2}
